\documentclass[preview]{standalone}

\usepackage{amsmath}
\usepackage{amsthm}
\usepackage{amsfonts}
\usepackage{mathtools}

\usepackage{hyperref}
\usepackage{cleveref}

\begin{document}

For output unit, based on textbook:

\begin{align}
\label{o0}
\frac{\partial E_d}{\partial net_j}=\frac{\partial E_d}{\partial o_j}\frac{\partial o_j}{\partial net_j}
\end{align}

Consider the first term:

\begin{align}
\label{o1}
\begin{split}
\frac{\partial E_d}{\partial o_j}
&=\frac{\partial}{\partial o_j}\frac{1}{2}\sum_d(t_d-o_d)^2\qquad\texttt{//only $d = j$ matters}\\
&=\frac{\partial}{\partial o_j}\frac{1}{2}(t_j-o_j)^2\\
&=\frac{1}{2} \cdot 2 \cdot (t_j-o_j)\frac{\partial(t_j-o_j)}{\partial o_j}\\
&=-(t_j-o_j)
\end{split}
\end{align}

Consider the second term, since the \texttt{identity} function is used, the
derivative is just the derivative of the \texttt{identity} function, which is
$1$.

\begin{align}
\label{o2}
\begin{split}
\frac{\partial o_j}{\partial net_j}=\frac{\partial}{\partial net_j}\mathtt{identity}(net_j) = 1
\end{split}
\end{align}

Substituting \cref{o1} and \cref{o2} into \cref{o0}:

\begin{align}
    \frac{\partial E_d}{\partial net_j}=-(t_j-o_j)
\end{align}

Thus, the gradient descent rule for output units is:

\begin{align}
\Delta w_{ji} = -\eta\frac{\partial E_d}{\partial w_{ji}} = \eta \cdot
(t_j-o_j) \cdot x_{ji}
\end{align}

\end{document}
