\documentclass[preview]{standalone}

\usepackage{amsmath}
\usepackage{amsthm}
\usepackage{amsfonts}
\usepackage{mathtools}

\begin{document}

\section{}

The training rule should be:

\begin{align}
    w_i\leftarrow w_i + \Delta w_i
\end{align}

where

\begin{align}
    \Delta w_i = -\eta\frac{\partial E}{\partial w_i}
\end{align}

We can calculate $\frac{\partial E}{\partial w_i}$ as follow:

\begin{align}
\begin{split}
\frac{\partial E}{\partial w_i}
&= \frac{\partial}{\partial w_i}\frac{1}{2}\sum_d(t_d-o_d)^2\\
&= \frac{1}{2}\sum_d\frac{\partial}{\partial w_i}(t_d-o_d)^2\\
&= \frac{1}{2}\sum_d2(t_d-o_d)\frac{\partial}{\partial w_i}(t_d-o_d)\\
&= \sum_d(t_d-o_d)\frac{\partial}{\partial w_i}(t_d-\vec{w}\cdot(\vec{x_d}+\vec{x_d}^2))\\
\frac{\partial E}{\partial w_i}
&= \sum_d(t_d-o_d)(-x_{i,d}-x_{i,d}^2)
\end{split}
\end{align}

Thus, we have:

\begin{align}
    \Delta w_i = \eta \sum_{d\in D} (t_d - i_d)(x_{i,d}+x_{i,d}^2)
\end{align}
\qed
\end{document}
