\documentclass[preview]{standalone}

\usepackage{amsmath}
\usepackage{amsthm}
\usepackage{amsfonts}
\usepackage{mathtools}
\usepackage{cleveref}

\begin{document}

\section{}

\subsection{}

First calculate $x_3$ and $x_4$:

\[x_3 = w_{31} x_1 + w_{32} x_2\]
\[x_4 = w_{41} x_1 + w_{42} x_2\]

Then, $x_5$:

\begin{align}
\begin{split}
x_5 &= w_{53} h(x_3) + w_{54} h(x_4)\\
    &= w_{53} h(w_{31} x_1 + w_{32} x_2) + w_{54} h(w_{41} x_1 + w_{42} x_2)
\end{split}
\end{align}

Final output would be:

\begin{align}
\begin{split}
o
&= h(x_5)\\
&= h(w_{53} h(w_{31} x_1 + w_{32} x_2) + w_{54} h(w_{41} x_1 + w_{42} x_2))
\end{split}
\end{align}

\subsection{}

If vector notation is used:

\begin{align}
    \label{nn1}
    o = W^{(2)} \cdot h(W^{(1)} \cdot X)
\end{align}

\subsection{}

Basically, we can transform $h_2(x)$ as:

\begin{align}
\begin{split}
    h_2(x) &= \frac{e^x-e^{-x}}{e^x+e^{-x}}\\
           &= \frac{e^x-e^{-x}}{e^x+e^{-x}} + 1 - 1\\
           &= \frac{e^x-e^{-x} + e^x + e^{-x}}{e^x+e^{-x}} - 1\\
           &= \frac{2e^x}{e^x+e^{-x}} - 1\\
           &= \frac{2}{1+e^{-2x}} - 1\\
    h_2(x) &= 2h_1(2x)-1
\end{split}
\end{align}

Substitute into \cref{nn1}:

\begin{align}
\begin{split}
o &= W^{(2)} \cdot h_2(W^{(1)} \cdot X) \\
  &= W^{(2)} \cdot2h_1(W^{(1)} \cdot 2 \cdot X) - 1
\end{split}
\end{align}

Basically it is same function.

\qed
\end{document}
